src/rocq/Semantics/LLVMEvents.v
@@ -83,6 +83,57 @@ Section withParams.
     | StackRaise      : exc -> StackE unit             (* Place exception onto the stack, does not pop *)
     | StackGetExc     : StackE (option exc).          (* Fetches the currently raised exception if there is one *)
 
+  (* Interactions with the memory *)
+  Variant MemoryE : Type -> Type :=
+    | MemPush : MemoryE unit
+    | MemPop  : MemoryE unit
+    | Alloca  (t : dtyp) (num_elements : N) (align : option Z) :
+      MemoryE dvalue
+    (* Load address should also be unique *)
+    | Load   (t : dtyp) (a : dvalue) :
+      MemoryE dvalue
+    (* Store address should be unique... *)
+    | Store (t : dtyp) (a : dvalue) (v : dvalue) :
+      MemoryE unit.
+
+  (* An event resolving the non-determinism induced by undef. The argument _P_
+   is intended to be a predicate over the set of dvalues _u_ can take such that
+   if it is not satisfied, the only possible execution is to raise _UB_. *)
+  Variant DrawE : Type -> Type :=
+    | draw (dt : dtyp) : DrawE dvalue.
+
+    (* Generic calls, refined by [denote_mcfg] *)
+  Variant CallE : Type -> Type :=
+    | Call        : forall (t:dtyp) (f:dvalue) (args:list dvalue), CallE (exc + dvalue).
+
+  (* ExternalCallE values are the "observable" events by which one should compare the 
+       equivalence of two LLVM IR programs.  These should never be interpreted away
+       by the Coq semantics. However, for practicality, we _do_ interpet some calls that
+       generate outputs to [stdout] (SAZ: and eventuall[stderr]).  The stream of bytes
+       visible in [IO_stdout] events is the data printed to [stdout].
+
+       - [ExternalCall] represents interactions with the OS
+       - [IO_stdout] represents bytes sent to [stdout]
+       - [IO_stderr] represents bytes sent to [stderr]
+
+       The latter two are actually printed to the console by [interpreter.ml]
+   *)
+  Variant ExternalCallE : Type -> Type :=
+    | ExternalCall (t : dtyp) (f : dvalue) (args : list dvalue) :
+      ExternalCallE dvalue
+    (* This event corresponds to writing to the [stdout] channel. ] *)                              
+    | IO_stdout (str : list int8) :
+      ExternalCallE unit
+    (* This event corresponds to writing to the [stderr] channel. ] *)                              
+    | IO_stderr (str : list int8) :
+      ExternalCallE unit.
+
+  (* Call to an intrinsic whose implementation do not rely on the implementation of the memory model *)
+  (* Intrinsics may raise an exception by returning inl *)
+  Variant IntrinsicE : Type -> Type :=
+    | Intrinsic (t : dtyp) (f : string) (args : list dvalue) :
+      IntrinsicE (exc + dvalue).
+  
   (* LLVM exceptions *)
   Variant LLVMExcE : Type -> Type :=
     | LLVMExc : exc -> LLVMExcE void.
@@ -98,11 +149,12 @@ Section withParams.
         force extraction 
       - print_msg call `print_string`
    *)
-  Record printer := mk_printer {
-      printer_set_loc : string -> string ;
-      printer_print_msg : string -> unit ;
-      printer_get_loc : unit -> string ;
-    }.
+  Record printer :=
+    mk_printer {
+        printer_set_loc : string -> string ;
+        printer_print_msg : string -> unit ;
+        printer_get_loc : unit -> string ;
+      }.
   
   Definition printer_object : printer :=
     mk_printer (fun (_:string) => "") (fun (_:string) => tt) (fun (_:unit) => "").
@@ -110,7 +162,7 @@ Section withParams.
   Definition set_loc : string -> string := printer_object.(printer_set_loc).
   Definition print_msg : string -> unit := printer_object.(printer_print_msg).
   Definition get_loc : unit -> string := printer_object.(printer_get_loc).
-
+ 
   (* Undefined behaviour carries a string. *)
   Variant UBE : Type -> Type :=
     | ThrowUB : unit -> UBE void.
@@ -120,6 +172,13 @@ Section withParams.
   Definition raiseUB {E : Type -> Type} `{UBE -< E} {X}
     (e : string) : itree E X :=
     v <- trigger (ThrowUB (print_msg e));; match v: void with end.
+
+  (* Failure. Carries a string for a message. *)
+  Variant FailureE : Type -> Type :=
+    | Throw : unit -> FailureE void.
+
+  Definition raise {E} {A} `{FailureE -< E} (msg : string) : itree E A :=
+    v <- trigger (Throw (print_msg msg));; match v: void with end.
 
   (* Out of memory / abort. Carries a string for a message. *)
   Variant OOME : Type -> Type :=
@@ -140,486 +199,114 @@ Section withParams.
   Definition debug {E} `{DebugE -< E} (msg : string) : itree E unit :=
     trigger (Debug (print_msg msg)).
 
-  (* Failure. Carries a string for a message. *)
-  Variant FailureE : Type -> Type :=
-    | Throw : unit -> FailureE void.
-
-  Definition raise {E} {A} `{FailureE -< E} (msg : string) : itree E A :=
-    v <- trigger (Throw (print_msg msg));; match v: void with end.
-
-  Section Events.
-    
-    (* Generic calls, refined by [denote_mcfg] *)
-    Variant CallE : Type -> Type :=
-      | Call        : forall (t:dtyp) (f:dvalue) (args:list dvalue), CallE (exc + dvalue).
-
-    (* ExternalCallE values are the "observable" events by which one should compare the 
-       equivalence of two LLVM IR programs.  These should never be interpreted away
-       by the Coq semantics. However, for practicality, we _do_ interpet some calls that
-       generate outputs to [stdout] (SAZ: and eventuall[stderr]).  The stream of bytes
-       visible in [IO_stdout] events is the data printed to [stdout].
-
-       - [ExternalCall] represents interactions with the OS
-       - [IO_stdout] represents bytes sent to [stdout]
-       - [IO_stderr] represents bytes sent to [stderr]
-
-       The latter two are actually printed to the console by [interpreter.ml]
-     *)
-    Variant ExternalCallE : Type -> Type :=
-      | ExternalCall (t : dtyp) (f : dvalue) (args : list dvalue) :
-        ExternalCallE dvalue
-      (* This event corresponds to writing to the [stdout] channel. ] *)                              
-      | IO_stdout (str : list int8) :
-        ExternalCallE unit
-      (* This event corresponds to writing to the [stderr] channel. ] *)                              
-      | IO_stderr (str : list int8) :
-        ExternalCallE unit.
-
-    (* Call to an intrinsic whose implementation do not rely on the implementation of the memory model *)
-    (* Intrinsics may raise an exception by returning inl *)
-    Variant IntrinsicE : Type -> Type :=
-      | Intrinsic (t : dtyp) (f : string) (args : list dvalue) :
-        IntrinsicE (exc + dvalue).
-
-    (* Interactions with the memory *)
-    Variant MemoryE : Type -> Type :=
-      | MemPush : MemoryE unit
-      | MemPop  : MemoryE unit
-      | Alloca  (t : dtyp) (num_elements : N) (align : option Z) :
-        MemoryE dvalue
-      (* Load address should also be unique *)
-      | Load   (t : dtyp) (a : dvalue) :
-        MemoryE dvalue
-      (* Store address should be unique... *)
-      | Store (t : dtyp) (a : dvalue) (v : dvalue) :
-        MemoryE unit.
-
-    (* An event resolving the non-determinism induced by undef. The argument _P_
-   is intended to be a predicate over the set of dvalues _u_ can take such that
-   if it is not satisfied, the only possible execution is to raise _UB_. *)
-    Variant DrawE : Type -> Type :=
-      | draw (dt : dtyp) : DrawE dvalue.
-    
-    (* The signatures for computations that we will use during the successive stages of the interpretation of LLVM programs *)
-    (* TODO: The events and handlers are parameterized by the types of key and value.
-     It's weird for it to be the case if the events are concretely instantiated right here.
-     At least TODO: remove these prefixes that are inconsistent with other names.
-     *)
-    Definition conv_E := MemoryE +' DrawE +' OOME +' LLVMExcE +' UBE +' DebugE +' FailureE.
-    Definition lookup_E := GlobalE +' LocalE.
-    Definition exp_E := GlobalE +' LocalE +' MemoryE +' DrawE +' OOME +' LLVMExcE +' UBE +' DebugE +' FailureE.
-
-    Definition LU_to_exp : lookup_E ~> exp_E :=
-      fun T e =>
-        match e with
-        | inl1 e => inl1 e
-        | inr1 e => inr1 (inl1 e)
-        end.
-
-    Definition conv_to_exp : conv_E ~> exp_E :=
-      fun T e => inr1 (inr1 e).
-
-    Definition instr_E := CallE +' IntrinsicE +' exp_E.
-    Definition exp_to_instr : exp_E ~> instr_E :=
-      fun T e => subevent _ e.
-
   (* Core effects. *)
   Definition L0' := CallE +' ExternalCallE +' IntrinsicE +' GlobalE +' (LocalE +' StackE) +' MemoryE +' DrawE +' OOME +' LLVMExcE +' UBE +' DebugE +' FailureE.
-
-  Definition instr_to_L0' : instr_E ~> L0' := subevent.
-
-  Definition exp_to_L0' : exp_E ~> L0' := subevent.
-
-  Definition FUB_to_exp : (FailureE +' UBE) ~> exp_E := subevent.
-
-  Definition FUBO_to_exp : (FailureE +' UBE +' OOME) ~> exp_E := subevent.
-
-  Definition L0 := ExternalCallE +' IntrinsicE +' GlobalE +' (LocalE +' StackE) +' MemoryE +' DrawE +' OOME +' LLVMExcE +' UBE +' DebugE +' FailureE.
-
-  Definition exp_to_L0 : exp_E ~> L0 := subevent.
-
-  (* For multiple CFG, after interpreting [GlobalE] *)
-  Definition L1 := ExternalCallE +' IntrinsicE +' (LocalE +' StackE) +' MemoryE +' DrawE +' OOME +' LLVMExcE +' UBE +' DebugE +' FailureE.
-
-  (* For multiple CFG, after interpreting [LocalE] *)
-  Definition L2 := ExternalCallE +' IntrinsicE +' MemoryE +' DrawE +' OOME +' LLVMExcE +' UBE +' DebugE +' FailureE.
-
-  (* For multiple CFG, after interpreting [LocalE] and [MemoryE] and [IntrinsicE] that are memory intrinsics *)
-  Definition L3 := ExternalCallE +' DrawE +' OOME +' LLVMExcE +' UBE +' DebugE +' FailureE.
+  Definition L0  :=          ExternalCallE +' IntrinsicE +' GlobalE +' (LocalE +' StackE) +' MemoryE +' DrawE +' OOME +' LLVMExcE +' UBE +' DebugE +' FailureE.
 
   (* For multiple CFG, after interpreting [LocalE] and [MemoryE] and [IntrinsicE] that are memory intrinsics and [DrawE]*)
-  (* Interprets [Pick] events: forcing evaluation of [dvalue]s, [UBE] has no semantic meaning *)
-  Definition L4 := ExternalCallE +' OOME +' LLVMExcE +' UBE +' DebugE +' FailureE.
+  (* Interprets [Draw] events: forcing evaluation of [dvalue]s, [UBE] has no semantic meaning *)
+  Definition L1 := ExternalCallE +' OOME +' LLVMExcE +' UBE +' DebugE +' FailureE.
 
-  (* [UBE] is still present in tree to identify failure, but the [model_UB] semantics allows [UB] to subsume all behavior *)
-  Definition L5 := ExternalCallE +' OOME +' LLVMExcE +' UBE +' DebugE +' FailureE.
-
-  (* [OOM] semantics is introduced through [interp_prop], so the semantic change is not apparent in the event signature *)
-  Definition L6 := ExternalCallE +' OOME +' LLVMExcE +' UBE +' DebugE +' FailureE.
-
-  Definition FUBO_to_L4 : (FailureE +' UBE +' OOME) ~> L4:= subevent.
-
-
-  
-  (* Event Inclusions -------------------------------- *)
-
-  #[global]
-    Instance Global_lookup : GlobalE -< lookup_E :=
-    inl1.
-
-  #[global]
-    Instance Local_lookup : LocalE -< lookup_E :=
-    inr1.
-
-  
-  (* expE *)
-  (*   Definition exp_E := LLVMGEnvE +' LocalE +' MemoryE +' DrawE +' OOME +' LLVMExcE dvalue +' UBE +' DebugE +' FailureE. *)
-  #[global]
-    Instance Failure_expE : `{FailureE -< exp_E} := 
-    fun T e => (inr1 (inr1 (inr1 (inr1 (inr1 (inr1 (inr1 (inr1 e)))))))).
-
-  #[global]
-    Instance DebugE_expE : `{DebugE -< exp_E} := 
-    fun T e => (inr1 (inr1 (inr1 (inr1 (inr1 (inr1 (inr1 (inl1 e)))))))).
-
-  #[global]
-    Instance UBE_expE : `{UBE -< exp_E} := 
-    fun T e => (inr1 (inr1 (inr1 (inr1 (inr1 (inr1 (inl1 e))))))).
-
-  #[global]
-    Instance LLVMExcE_expE : `{LLVMExcE -< exp_E} := 
-    fun T e => (inr1 (inr1 (inr1 (inr1 (inr1 (inl1 e)))))).
-  
-  #[global]
-    Instance OOME_expE : `{OOME -< exp_E} := 
-    fun T e => (inr1 (inr1 (inr1 (inr1 (inl1 e))))).
-
-  #[global]
-    Instance PickE_expE : `{DrawE -< exp_E} := 
-    fun T e => (inr1 (inr1 (inr1 (inl1 e)))).
-
-  #[global]
-    Instance MemoryE_expE : `{MemoryE -< exp_E} := 
-    fun T e => (inr1 (inr1 (inl1 e))).
-
-  #[global]
-    Instance LocalE_expE : `{LocalE -< exp_E} := 
-    fun T e => (inr1 (inl1 e)).
-
-  #[global]
-    Instance GlobalE_expE : `{GlobalE -< exp_E} := 
-    fun T e => (inl1 e).
-
-  (* instr_E *)
-  
-  #[global]
-    Instance Failure_instrE : `{FailureE -< instr_E} := 
-    fun T e => (inr1 (inr1 (Failure_expE e))).
-
-  #[global]
-    Instance DebugE_instrE : `{DebugE -< instr_E} := 
-    fun T e => (inr1 (inr1 (DebugE_expE e))).
-  
-  #[global]
-    Instance UBE_instrE : `{UBE -< instr_E} := 
-    fun T e => (inr1 (inr1 (UBE_expE e))).
-
-  #[global]
-    Instance LLVMExcE_instrE : `{LLVMExcE -< instr_E } := 
-    fun T e => (inr1 (inr1 (LLVMExcE_expE e))).
-  
-  #[global]
-    Instance OOME_instrE : `{OOME -< instr_E} := 
-    fun T e => (inr1 (inr1 (OOME_expE e))).
-
-  #[global]
-    Instance PickE_instrE : `{DrawE -< instr_E} := 
-    fun T e => (inr1 (inr1 (PickE_expE e))).
-
-  #[global]
-    Instance MemoryE_instrE : `{MemoryE -< instr_E} := 
-    fun T e => (inr1 (inr1 (MemoryE_expE e))).
-
-  #[global]
-    Instance LocalE_instrE : `{LocalE -< instr_E } := 
-    fun T e => (inr1 (inr1 (LocalE_expE e))).
-  
-  #[global]
-    Instance GlobalE_instrE : `{GlobalE -< instr_E } := 
-    fun T e => (inr1 (inr1 (GlobalE_expE e))).
-
-  #[global]
-    Instance IntrinsicE_instrE : `{IntrinsicE -< instr_E } := 
-    fun T e => (inr1 (inl1 e)).
-
-  #[global]
-    Instance CallE_instrE : `{CallE -< instr_E} := 
-    fun T e => (inl1 e).
-
-  (* L0' *)
-  (*   Definition L0' := CallE +' ExternalCallE +' IntrinsicE +' GlobalE +' (LocalE +' StackE) +' MemoryE +' DrawE +' OOME +' LLVMExcE dvalue +' UBE +' DebugE +' FailureE. *)
-
-  #[global]
-    Instance FailureE_L0' : `{FailureE -< L0'} := 
+  (* TODO: Test if these have any sensible impact *)
+  #[global] Instance FailureE_L0' : `{FailureE -< L0'} := 
     fun T e => inr1 (inr1 (inr1 (inr1 (inr1 (inr1 (inr1 (inr1 (inr1 (inr1 (inr1 e)))))))))).
 
-  #[global]
-    Instance DebugE_L0' : `{DebugE -< L0'} := 
+  #[global] Instance DebugE_L0' : `{DebugE -< L0'} := 
     fun T e => inr1 (inr1 (inr1 (inr1 (inr1 (inr1 (inr1 (inr1 (inr1 (inr1 (inl1 e)))))))))).
   
-  #[global]
-    Instance UBE_L0' : UBE -< L0' :=
+  #[global] Instance UBE_L0' : UBE -< L0' :=
     fun T e => (inr1 (inr1 (inr1 (inr1 (inr1 (inr1 (inr1 (inr1 (inr1 (inl1 e)))))))))).
 
-  #[global]
-    Instance LLVMExcE_L0' : LLVMExcE -< L0' :=
+  #[global] Instance LLVMExcE_L0' : LLVMExcE -< L0' :=
     fun T e => (inr1 (inr1 (inr1 (inr1 (inr1 (inr1 (inr1 (inr1 (inl1 e))))))))).
   
-  #[global]
-    Instance OOME_L0' : OOME -< L0' :=
+  #[global] Instance OOME_L0' : OOME -< L0' :=
     fun T e => (inr1 (inr1 (inr1 (inr1 (inr1 (inr1 (inr1 (inl1 e)))))))).
 
-  #[global]
-    Instance DrawE_L0' : DrawE -< L0' :=
+  #[global] Instance DrawE_L0' : DrawE -< L0' :=
     fun T e => (inr1 (inr1 (inr1 (inr1 (inr1 (inr1 (inl1 e))))))).
   
-    #[global]
-    Instance MemoryE_L0' : `{MemoryE -< L0'} := 
+  #[global] Instance MemoryE_L0' : `{MemoryE -< L0'} := 
     fun T e => (inr1 (inr1 (inr1 (inr1 (inr1 (inl1 e)))))).
 
-  #[global]
-    Instance LocalE_L0' : `{LocalE  -< L0'} := 
+  #[global] Instance LocalE_L0' : `{LocalE  -< L0'} := 
     fun T e => inr1 (inr1 (inr1 (inr1 (inl1 (inl1 e))))).
 
-  #[global]
-    Instance StackE_L0' : `{StackE  -< L0'} := 
+  #[global] Instance StackE_L0' : `{StackE  -< L0'} := 
     fun T e => inr1 (inr1 (inr1 (inr1 (inl1 (inr1 e))))).
 
-  #[global]
-    Instance GEnvE_L0' : `{GlobalE  -< L0'} := 
+  #[global] Instance GEnvE_L0' : `{GlobalE  -< L0'} := 
     fun T e => (inr1 (inr1 (inr1 (inl1 e)))).
 
-  #[global]
-    Instance IntrinsicE_L0' : `{IntrinsicE  -< L0'} := 
+  #[global] Instance IntrinsicE_L0' : `{IntrinsicE  -< L0'} := 
     fun T e => (inr1 (inr1 (inl1 e))).
 
-  #[global]
-    Instance ExternalCallE_L0' : `{ExternalCallE  -< L0'} := 
+  #[global] Instance ExternalCallE_L0' : `{ExternalCallE  -< L0'} := 
     fun T e => (inr1 (inl1 e)).
 
-  #[global]
-    Instance CallE_L0' : `{CallE  -< L0'} := 
+  #[global] Instance CallE_L0' : `{CallE  -< L0'} := 
     fun T e => (inl1 e).
 
   (* L0 *)
-  (*   Definition L0 := ExternalCallE +' IntrinsicE +' GlobalE +' (LocalE +' StackE) +' MemoryE +' DrawE +' OOME +' LLVMExcE dvalue +' UBE +' DebugE +' FailureE. *)
 
-  #[global]
-    Instance FailureE_L0 : FailureE -< L0 :=
+  #[global] Instance FailureE_L0 : FailureE -< L0 :=
     fun T e => (inr1 (inr1 (inr1 (inr1 (inr1 (inr1 (inr1 (inr1 (inr1 (inr1 e)))))))))).
 
-  #[global]
-    Instance DebugE_L0 : DebugE -< L0 :=
+  #[global] Instance DebugE_L0 : DebugE -< L0 :=
     fun T e => (inr1 (inr1 (inr1 (inr1 (inr1 (inr1 (inr1 (inr1 (inr1 (inl1 e)))))))))).
 
-  #[global]
-    Instance UBE_L0 : UBE -< L0 :=
+  #[global] Instance UBE_L0 : UBE -< L0 :=
     fun T e => (inr1 (inr1 (inr1 (inr1 (inr1 (inr1 (inr1 (inr1 (inl1 e))))))))).
 
-  #[global]
-    Instance LLVMExcE_L0 : LLVMExcE -< L0 :=
+  #[global] Instance LLVMExcE_L0 : LLVMExcE -< L0 :=
     fun T e => (inr1 (inr1 (inr1 (inr1 (inr1 (inr1 (inr1 (inl1 e)))))))).
   
-  #[global]
-    Instance OOME_L0 : OOME -< L0  :=
+  #[global] Instance OOME_L0 : OOME -< L0  :=
     fun T e => inr1 (inr1 (inr1 (inr1 (inr1 (inr1 (inl1 e)))))).
 
-  #[global]
-    Instance DrawE_L0 : DrawE -< L0 :=
+  #[global] Instance DrawE_L0 : DrawE -< L0 :=
     fun T e => inr1 (inr1 (inr1 (inr1 (inr1 (inl1 e))))).
   
-  #[global]
-    Instance MemoryE_L0 : MemoryE  -< L0 :=
+  #[global] Instance MemoryE_L0 : MemoryE  -< L0 :=
     fun T e => inr1 (inr1 (inr1 (inr1 (inl1 e)))).
 
-  #[global]
-    Instance LocalE_expE_L0 : LocalE -< L0 :=
+  #[global] Instance LocalE_expE_L0 : LocalE -< L0 :=
     fun T e => inr1 (inr1 (inr1 (inl1 (inl1 e)))).
 
-  #[global]
-    Instance StackE_expE_L0 : StackE -< L0 :=
+  #[global] Instance StackE_expE_L0 : StackE -< L0 :=
     fun T e => inr1 (inr1 (inr1 (inl1 (inr1 e)))).
   
-  #[global]
-    Instance GlobalE_L0 : GlobalE -< L0 :=
+  #[global] Instance GlobalE_L0 : GlobalE -< L0 :=
     fun T e => (inr1 (inr1 (inl1 e))).
 
-  #[global]
-    Instance IntrinsincE_L0 : IntrinsicE -< L0 :=
+  #[global] Instance IntrinsincE_L0 : IntrinsicE -< L0 :=
     fun T e => (inr1 (inl1 e)).
 
-  #[global]
-    Instance ExternalCallE_L0 : ExternalCallE -< L0 :=
+  #[global] Instance ExternalCallE_L0 : ExternalCallE -< L0 :=
     fun T e => (inl1 e).
-
-
-  #[global]
-    Instance IntrinsiceE_expE_L0 : IntrinsicE  +' exp_E -< L0  :=
-    fun T e =>
-      match e with
-      | inl1 e => inr1 (inl1 e)
-      | inr1 e => exp_to_L0 e
-      end.
-
-
+  
   (* L1 *)
-  (*     Definition L1 := ExternalCallE +' IntrinsicE +' (LocalE +' StackE) +' MemoryE +' DrawE +' OOME +' LLVMExcE dvalue +' UBE +' DebugE +' FailureE. *)
 
-  #[global]
-    Instance FailureE_L1 : FailureE -< L1 :=
-    fun T e => (inr1 (inr1 (inr1 (inr1 (inr1 (inr1 (inr1 (inr1 (inr1 e))))))))).
-
-  #[global]
-    Instance DebugE_L1 : DebugE -< L1 :=
-    fun T e => (inr1 (inr1 (inr1 (inr1 (inr1 (inr1 (inr1 (inr1 (inl1 e))))))))).
-
-  #[global]
-    Instance UBE_L1 : UBE -< L1 :=
-    fun T e => (inr1 (inr1 (inr1 (inr1 (inr1 (inr1 (inr1 (inl1 e)))))))).
-
-  #[global]
-    Instance LLVMExcE_L1 : LLVMExcE -< L1 :=
-    fun T e => (inr1 (inr1 (inr1 (inr1 (inr1 (inr1 (inl1 e))))))).
-  
-  #[global]
-    Instance OOME_L1 : OOME -< L1  :=
-    fun T e => (inr1 (inr1 (inr1 (inr1 (inr1 (inl1 e)))))).
-
-  #[global]
-    Instance DrawE_L1 : DrawE -< L1 :=
-    fun T e => (inr1 (inr1 (inr1 (inr1 (inl1 e))))).
-  
-  #[global]
-    Instance MemoryE_L1 : MemoryE  -< L1 :=
-    fun T e => (inr1 (inr1 (inr1 (inl1 e)))).
-
-  #[global]
-    Instance LocalE_expE_L1 : LocalE -< L1 :=
-    fun T e => (inr1 (inr1 (inl1 (inl1 e)))).
-
-  #[global]
-    Instance StackE_expE_L1 : StackE -< L1 :=
-    fun T e =>  (inr1 (inr1 (inl1 (inr1 e)))).
-  
-  #[global]
-    Instance IntrinsincE_L1 : IntrinsicE -< L1 :=
-    fun T e => (inr1 (inl1 e)).
-
-  #[global]
-    Instance ExternalCallE_L1 : ExternalCallE -< L1 :=
-    fun T e => (inl1 e).
-
-  (* L2 *)
-  (* ExternalCallE +' IntrinsicE +' MemoryE +' DrawE +' OOME +' LLVMExcE dvalue +' UBE +' DebugE +' FailureE.    *)
-
-  #[global]
-    Instance FailureE_L2 : FailureE -< L2 :=
-    fun T e => (inr1 (inr1 (inr1 (inr1 (inr1 (inr1 (inr1 (inr1 e)))))))).
-
-  #[global]
-    Instance DebugE_L2 : DebugE -< L2 :=
-    fun T e => (inr1 (inr1 (inr1 (inr1 (inr1 (inr1 (inr1 (inl1 e)))))))).
-
-  #[global]
-    Instance UBE_L2 : UBE -< L2 :=
-    fun T e => (inr1 (inr1 (inr1 (inr1 (inr1 (inr1 (inl1 e))))))).
-
-  #[global]
-    Instance LLVMExcE_L2 : LLVMExcE -< L2 :=
-    fun T e => (inr1 (inr1 (inr1 (inr1 (inr1 (inl1 e)))))).
-  
-  #[global]
-    Instance OOME_L2 : OOME -< L2  :=
-    fun T e => (inr1 (inr1 (inr1 (inr1 (inl1 e))))).
-
-  #[global]
-    Instance DrawE_L2 : DrawE -< L2 :=
-    fun T e => (inr1 (inr1 (inr1 (inl1 e)))).
-  
-  #[global]
-    Instance MemoryE_L2 : MemoryE  -< L2 :=
-    fun T e => (inr1 (inr1 (inl1 e))).
-
-  #[global]
-    Instance IntrinsincE_L2 : IntrinsicE -< L2 :=
-    fun T e => (inr1 (inl1 e)).
-
-  #[global]
-    Instance ExternalCallE_L2 : ExternalCallE -< L2 :=
-    fun T e => (inl1 e).
-
-
-    (* L3 *)
-  (* ExternalCallE +' DrawE +' OOME +' LLVMExcE dvalue +' UBE +' DebugE +' FailureE. *)
-
-  #[global]
-    Instance FailureE_L3 : FailureE -< L3 :=
-    fun T e => (inr1 (inr1 (inr1 (inr1 (inr1 (inr1 e)))))).
-
-  #[global]
-    Instance DebugE_L3 : DebugE -< L3 :=
-    fun T e =>  (inr1 (inr1 (inr1 (inr1 (inr1 (inl1 e)))))).
-
-  #[global]
-    Instance UBE_L3 : UBE -< L3 :=
-    fun T e =>  (inr1 (inr1 (inr1 (inr1 (inl1 e))))).
-
-  #[global]
-    Instance LLVMExcE_L3 : LLVMExcE -< L3 :=
-    fun T e =>  (inr1 (inr1 (inr1 (inl1 e)))).
-  
-  #[global]
-    Instance OOME_L3 : OOME -< L3  :=
-    fun T e =>  (inr1 (inr1 (inl1 e))).
-
-  #[global]
-    Instance DrawE_L3 : DrawE -< L3 :=
-    fun T e =>  (inr1 (inl1 e)).
-  
-  #[global]
-    Instance ExternalCallE_L3 : ExternalCallE -< L3 :=
-    fun T e => (inl1 e).
-
-    (* L4 *)
-  (* ExternalCallE +' OOME +' LLVMExcE dvalue +' UBE +' DebugE +' FailureE. *)
-
-  #[global]
-    Instance FailureE_L4 : FailureE -< (ExternalCallE +' OOME +' LLVMExcE +' UBE +' DebugE +' FailureE) :=
+  #[global] Instance FailureE_L4 : FailureE -< (ExternalCallE +' OOME +' LLVMExcE +' UBE +' DebugE +' FailureE) :=
     fun T e => (inr1 (inr1 (inr1 (inr1 (inr1 e))))).
 
-  #[global]
-    Instance DebugE_L4 : DebugE -< (ExternalCallE +' OOME +' LLVMExcE +' UBE +' DebugE +' FailureE) :=
+  #[global] Instance DebugE_L4 : DebugE -< (ExternalCallE +' OOME +' LLVMExcE +' UBE +' DebugE +' FailureE) :=
     fun T e =>  (inr1 (inr1 (inr1 (inr1 (inl1 e))))).
 
-  #[global]
-    Instance UBE_L4 : UBE -< (ExternalCallE +' OOME +' LLVMExcE +' UBE +' DebugE +' FailureE) :=
+  #[global] Instance UBE_L4 : UBE -< (ExternalCallE +' OOME +' LLVMExcE +' UBE +' DebugE +' FailureE) :=
     fun T e =>  (inr1 (inr1 (inr1 (inl1 e)))).
 
-  #[global]
-    Instance LLVMExcE_L4 : LLVMExcE -< (ExternalCallE +' OOME +' LLVMExcE +' UBE +' DebugE +' FailureE) :=
+  #[global] Instance LLVMExcE_L4 : LLVMExcE -< (ExternalCallE +' OOME +' LLVMExcE +' UBE +' DebugE +' FailureE) :=
     fun T e =>  (inr1 (inr1 (inl1 e))).
   
-  #[global]
-    Instance OOME_L4 : OOME -< (ExternalCallE +' OOME +' LLVMExcE +' UBE +' DebugE +' FailureE) :=
+  #[global] Instance OOME_L4 : OOME -< (ExternalCallE +' OOME +' LLVMExcE +' UBE +' DebugE +' FailureE) :=
     fun T e =>  (inr1 (inl1 e)).
 
-  #[global]
-    Instance ExternalCallE_L4 : ExternalCallE -< (ExternalCallE +' OOME +' LLVMExcE +' UBE +' DebugE +' FailureE) :=
+  #[global] Instance ExternalCallE_L4 : ExternalCallE -< (ExternalCallE +' OOME +' LLVMExcE +' UBE +' DebugE +' FailureE) :=
     fun T e => (inl1 e).
   
-  End Events.
 End withParams.
 
 Arguments DrawE {_} _.
 
-#[export] Hint Unfold L0 L0' L1 L2 L4 L4 L5 L6 : core.
+#[export] Hint Unfold L0 L0' L1 : core.
