src/rocq/Semantics/InterpretationStack.v
@@ -20,36 +20,22 @@ From Vellvm Require Import
 Section withParams.
   Context {Pa : Params}.
   Existing Instance MemoryModelPrimitivesV.
-             
-    (**
+  
+  (**
    Partial interpretations of the trees produced by the denotation of _VIR_ programs.
    The intent is to allow us to only interpret as many layers as needed
    to perform the required semantic reasoning, and lift for free the
    equivalence down the pipe.
    This gives us a _vertical_ notion of compositionality.
-     *)
+   *)
 
-    (* TODO: just make these types, instead of duplicating the definitions? *)
-    Definition interp_mcfg1 {R} (t: itree L0 R) g : itree L1 (global_env * R) :=
-      let dvalue_trace       := interp_intrinsics t in
-      let L1_trace           := interp_global dvalue_trace g in
-      L1_trace.
+  Definition Res X := (state * (stack_frame * stack * (global_env * X)))%type.
+  
+  Definition interp_mcfg {R} (t: itree L0 R) g l m : itree L1 (Res R)  :=
+    let t0 := interp_intrinsics t in
+    let t1 := interp_global t0 g in
+    let t2 := interp_local_stack t1 l in
+    let t3 := interp_memory t2 m in
+    interp_draw t3.
 
-    Definition interp_mcfg2 {R} (t: itree L0 R) (g : global_env) (l : stack_frame * stack) : itree L2 (stack_frame * stack * (global_env * R)) :=
-      let L1_trace       := interp_mcfg1 t g in
-      let L2_trace       := interp_local_stack L1_trace l in
-      L2_trace.
-
-    Definition interp_mcfg3 {R} (t: itree L0 R) (g : global_env) (l : stack_frame * stack) (m : state) :
-      itree L3 (state * (stack_frame * stack * (global_env * R))) :=
-      let L2_trace       := interp_mcfg2 t g l in
-      let L3_trace       := interp_memory L2_trace m in
-      L3_trace.
-
-    Definition interp_mcfg4 {R} (t: itree L0 R) (g : global_env) (l : stack_frame * stack) (m : state) :
-      itree L4 (state * (stack_frame * stack * (global_env * R))) :=
-      let L3_trace       := interp_mcfg3 t g l m in
-      let L4_trace       := interp_draw L3_trace in
-      L4_trace.
-    
 End withParams.
